coq/Termination.v
@@ -1,22 +1,19 @@
-Require Import Arith List.
+Require Import Arith List Omega.
 Require Import Defs.
 Import ListNotations.
 
+(* Definitions related to well-founded measures *)
+
 Definition headFrameSize (fr : l_frame) : nat :=
-  match fr with
-  | (_, _, suf) => List.length suf
-  end.
+  List.length (symbolsToProcess fr).
 
 Definition headFrameScore (fr : l_frame) (b : nat) (e : nat) : nat :=
   headFrameSize fr * (b ^ e).
 
 Definition tailFrameSize (fr : l_frame) : nat :=
-  match fr with
-  | (_, _, suf) =>
-    match suf with
-    | [] => 0
-    | _ :: suf' => List.length suf'
-    end
+  match (symbolsToProcess fr) with
+  | []        => 0
+  | _ :: suf' => List.length suf'
   end.
 
 Definition tailFrameScore (fr : l_frame) (b : nat) (e : nat) : nat :=
@@ -41,3 +38,96 @@ Definition rhsLengths (g : grammar) : list nat :=
 Definition maxRhsLength (g : grammar) : nat :=
   listMax (rhsLengths g).
 
+(* Termination-related lemmas *)
+
+Lemma nonzero_exponents_lt_powers_le :
+  forall b e1 e2, 0 < e1 < e2 -> b ^ e1 <= b ^ e2.
+Proof.
+  intros b e1 e2 [Hlt Hlt']. 
+  destruct b as [| b']. 
+  - destruct e1; destruct e2; auto.
+    omega.
+  - destruct b' as [| b''].
+    + repeat rewrite Nat.pow_1_l; auto.
+    + pose proof Nat.pow_lt_mono_r. 
+      specialize (H (S (S b'')) e1 e2). 
+      assert (fact : forall n m, n < m -> n <= m) by (intros; omega).
+      apply fact.
+      apply Nat.pow_lt_mono_r; auto.
+      omega.
+Qed.
+
+Lemma nonzero_exponents_lt_tailFrameScore_le :
+  forall fr b e1 e2,
+    0 < e1 < e2
+    -> tailFrameScore fr b e1 <= tailFrameScore fr b e2.
+Proof.
+  intros fr b e1 e2 Hlt.
+  unfold tailFrameScore. 
+  apply Nat.mul_le_mono_l.
+  apply nonzero_exponents_lt_powers_le; auto.
+Qed.
+
+Lemma nonzero_exponents_lt_tailFramesScore_le :
+  forall frs b e1 e2,
+    0 < e1 < e2
+    -> tailFramesScore frs b e1 <= tailFramesScore frs b e2.
+Proof.
+  intros frs.
+  induction frs as [| fr frs IH]; intros b e1 e2 Hlt; simpl; auto.
+  apply plus_le_compat.
+  - apply nonzero_exponents_lt_tailFrameScore_le; auto.
+  - apply IH; omega.
+Qed.
+
+Lemma nonzero_exponents_lt_stackScore_le :
+  forall v b e1 e2 e3 e4 frs,
+    0 < e1 < e2
+    -> 0 < e3 < e4
+    -> v * (b ^ e1) + tailFramesScore frs b e3 <= 
+       v * (b ^ e2) + tailFramesScore frs b e4.
+Proof.
+  intros v b e1 e2 e3 e4 frs [H0e1 He1e2] [H0e3 He3e4].
+  apply plus_le_compat.
+  - apply Nat.mul_le_mono_l. 
+    apply nonzero_exponents_lt_powers_le; auto.
+  - apply nonzero_exponents_lt_tailFramesScore_le; auto.
+Qed.
+
+Lemma mem_true_cardinality_neq_0 :
+  forall x s,
+    NtSet.mem x s = true -> NtSet.cardinal s <> 0.
+Proof.
+  intros x s Hm; unfold not; intros Heq.
+  rewrite NtSet.mem_spec in Hm.
+  apply cardinal_inv_1 in Heq.
+  unfold NtSet.Empty in Heq. 
+  eapply Heq; eauto.
+Qed.
+
+Lemma mem_true_cardinality_gt_0 :
+  forall x s,
+    NtSet.mem x s = true -> 0 < NtSet.cardinal s.
+Proof.
+  intros x s Hm.
+  apply mem_true_cardinality_neq_0 in Hm; omega.
+Qed.
+
+Lemma stackScore_le_after_return :
+  forall callee caller caller' x av frs b,
+    symbolsToProcess callee = []
+    -> symbolsToProcess caller = NT x :: symbolsToProcess caller'
+    -> stackScore (caller', frs) b (NtSet.cardinal (NtSet.add x av)) <= stackScore (callee, caller :: frs) b (NtSet.cardinal av).
+Proof.
+  intros callee caller caller' x av frs b Hcallee Hcaller.
+  unfold stackScore. 
+  unfold headFrameScore; unfold headFrameSize; rewrite Hcallee; simpl; clear Hcallee.
+  unfold tailFrameScore; unfold tailFrameSize; rewrite Hcaller; clear Hcaller.
+  destruct (NtSet.mem x av) eqn:Hm.
+  - rewrite add_cardinal_1; auto.
+    eapply nonzero_exponents_lt_stackScore_le.
+    + split; auto.
+      eapply mem_true_cardinality_gt_0; eauto.
+    + split; omega.
+  - rewrite add_cardinal_2; auto.
+Qed.
