coq/Lemmas.v
@@ -1,0 +1,11 @@
+Require Import List.
+Require Import Tactics.
+Import ListNotations.
+
+Lemma in_singleton_eq :
+  forall A (x x' : A), In x' [x] -> x' = x.
+Proof.
+  intros A x x' Hin.
+  destruct Hin as [Hhd | Htl]; auto.
+  inv Htl.
+Qed.
