coq/Tactics.v
@@ -1,1 +1,31 @@
 Ltac inv H := inversion H; subst; clear H.
+
+Ltac tc := try congruence.
+
+(* destruct a match in a hypothesis *)
+Ltac dmh := match goal with
+             | H : context[match ?x with | _ => _ end] |- _ => destruct x
+             end.
+
+(* destruct a match in the goal *)
+Ltac dmg := match goal with
+             | |- context[match ?x with | _ => _ end] => destruct x
+             end.
+
+Ltac dm  := (first [dmh | dmg]); auto.
+
+(* destruct a match in a hypothesis, and save the equality in the context *)
+Ltac dmh_eq s := let Heq := fresh s in
+                 match goal with
+                 | H : context[match ?x with | _ => _ end] |- _ =>
+                   destruct x eqn:Heq
+                 end.
+
+(* destruct a match in the goal, and save the equality in the context *)
+Ltac dmg_eq s := let Heq := fresh s in
+                 match goal with
+                 | |- context[match ?x with | _ => _ end] => destruct x eqn:Heq
+                 end.
+
+Ltac dmeq s := (first [dmh_eq s | dmg_eq s]); auto.
+
